Splinter/Message.s.dfy
@@ -1,40 +1,101 @@
 // Copyright 2018-2021 VMware, Inc., Microsoft Inc., Carnegie Mellon University, ETH Zurich, and University of Washington
 // SPDX-License-Identifier: BSD-2-Clause
 
+
+include "../lib/Base/KeyType.s.dfy"
 include "../lib/Lang/NativeTypes.s.dfy"
-//include "../lib/Base/total_order_impl.i.dfy"
+include "../lib/Lang/LinearSequence.s.dfy"
 
-// TODO replace this stuff with the real key, value, message definitions
-
-// Messages are high-level Ops over the Betree
-module MessageMod {
-
-  //import KeysImpl = Lexicographic_Byte_Order_Impl
-  //import Keys = KeysImpl.Ord
-
-  //type Key(!new) //= Keys.Element
-  type Key(!new,==) // TODO(sowmya): Message shouldn't have key, I think
+abstract module MessageMod {
   type Value(!new)
+  type Delta(!new)
 
-  //type Message(!new)
-  // TODO: Make Messages be more general either terminal updates or
-  datatype Message = MessagePut(v:Value)
+  function method NopDelta() : Delta
+  function method DefaultValue() : Value
 
-  predicate IsAKey(k: Key) { true }  // a term for Dafny to trigger on, to hide the warning.
+  datatype Message =
+    | Define(value: Value)
+    | Update(delta: Delta)
 
-  function AllKeys() : iset<Key> {
-    iset key:Key | IsAKey(key)
+  function method CombineDeltas(newdelta: Delta, olddelta: Delta) : (result: Delta)
+  ensures newdelta == NopDelta() ==> result == olddelta
+  ensures olddelta == NopDelta() ==> result == newdelta
+
+  function method ApplyDelta(delta: Delta, value: Value) : (result: Value)
+  ensures delta == NopDelta() ==> result == value
+
+  function method Merge(newmessage: Message, oldmessage: Message) : Message {
+    match (newmessage, oldmessage) {
+      case (Define(newvalue), _) => Define(newvalue)
+      case (Update(newdelta), Update(olddelta)) => Update(CombineDeltas(newdelta, olddelta))
+      case (Update(delta), Define(value)) => Define(ApplyDelta(delta, value))
+    }
   }
 
-  function DefaultValue() : Value
-    // TODO
+  function method IdentityMessage() : Message {
+    Update(NopDelta())
+  }
 
-  function DefaultMessage() : Message
+  function method DefaultMessage() : Message {
+    Define(DefaultValue())
+  }
+
+  lemma DeltaIsAssociative(a: Delta, b: Delta, c: Delta)
+    ensures CombineDeltas(CombineDeltas(a, b), c) == CombineDeltas(a, CombineDeltas(b, c))
+
+  lemma ApplyIsAssociative(a: Delta, b: Delta, value: Value)
+    ensures ApplyDelta(CombineDeltas(a, b), value) == ApplyDelta(a, ApplyDelta(b, value))
+
+  lemma MergeIsAssociative(a: Message, b: Message, c: Message)
+    ensures Merge(Merge(a, b), c) == Merge(a, Merge(b, c))
+    {
+      match a {
+        case Define(a) => { }
+        case Update(a) => {
+          match b {
+            case Define(b) => { }
+            case Update(b) => {
+              match c {
+                case Define(c) => {
+                  ApplyIsAssociative(a, b, c);
+                }
+                case Update(c) => {
+                  DeltaIsAssociative(a, b, c);
+                }
+              }
+            }
+          }
+        }
+      }
+    }
+}
+
+// No Delta Messages
+module ValueMessage refines MessageMod {
+  import ValueType`Internal
+  import opened NativeTypes
+  import opened LinearSequence_s
+  //import opened Sequences
+
+  type Value = ValueType.Value
+  datatype Delta = NoDelta
+
+  function method NopDelta() : Delta { NoDelta }
+  function method DefaultValue() : Value { ValueType.DefaultValue() }
+
+  function method CombineDeltas(newdelta: Delta, olddelta: Delta) : Delta { NoDelta }
+  function method ApplyDelta(delta: Delta, value: Value) : Value { value }
+
+  lemma DeltaIsAssociative(a: Delta, b: Delta, c: Delta)
   {
-    MessagePut(DefaultValue())
   }
 
-  // QUESTION: We use this to apply the key to map in msgSeq. Does this go here?
-  function Combine(oldMsg : Message, newMsg: Message) : Message
-   // TODO
+  lemma ApplyIsAssociative(a: Delta, b: Delta, value: Value)
+  {
+  }
+
+  predicate EncodableMessage(msg: Message)
+  {
+    && msg.Define?
+  }
 }
